src/ShouldBuild.v
@@ -1,6 +1,6 @@
 From Perennial Require Import program_logic.crash_lang.
 From Perennial Require Import program_logic.crash_weakestpre.
-(* From Perennial Require Import program_logic.spec_assert. *)
+From Perennial Require Import program_logic.spec_assert.
 From Perennial Require Import program_logic.recovery_adequacy.
 From Perennial Require Import program_logic.crash_inv.
 From Perennial Require Import heap_lang.crash_lock.
